module z02-theorem-proving-with-booleans where

open import bool
open import eq
open import level

-- p 28
~~tt : ~ ~ tt â‰¡ tt
~~tt = refl

-- p 32
~~ff : ~ ~ ff â‰¡ ff
~~ff = refl

-- p 33
~~-elim : âˆ€ (b : ğ”¹) â†’ ~ ~ b â‰¡ b
~~-elim tt = refl
~~-elim ff = refl

-- p 34
~~-elim2 : âˆ€ (b : ğ”¹) â†’ ~ ~ b â‰¡ b
~~-elim2 tt = ~~tt
~~-elim2 ff = ~~ff

{-
-- p 34 - does not typecheck (on purpose) because of IMPLICIT ARGS
-- IMPLICIT ARGS: stated inside curly brackets (like IF previously)
~~-elim3 : âˆ€ (b : ğ”¹) â†’ ~ ~ b â‰¡ b
~~-elim3 tt = ~~ff
~~-elim3 ff = ~~tt

'refl' has implicit args
- the expression 'x' in 'x â‰¡ x' (e.g., in ~~tt the implicit is 'tt')
  - in ~~-elim3 implicit arg 'tt' does not match '~~ff'
-}

{-
-- p 35 : HOLES

~~-elim4 : âˆ€ (b : ğ”¹) â†’ ~ ~ b â‰¡ b
~~-elim4 tt = ?
~~-elim4 ff = ?
-}

-- p 36
&&-same : âˆ€ (b : ğ”¹) â†’ b && b â‰¡ b
&&-same tt = refl
&&-same ff = refl

-- infer type of 'b'
&&-same2 : âˆ€ b â†’ b && b â‰¡ b
&&-same2 tt = refl
&&-same2 ff = refl

-- 'b' as implicit argument
&&-same3 : âˆ€ {b} â†’ b && b â‰¡ b
&&-same3 {tt} = refl
&&-same3 {ff} = refl

-- p 37
-- so no need to supply implicit arg to &&-same3
test-&&-same : tt && tt â‰¡ tt
test-&&-same = &&-same3

-- ok to explicitly supply implicit arg
test-&&-same2 : tt && tt â‰¡ tt
test-&&-same2 = &&-same3 {tt}

-- p 38
||-same : âˆ€ {b} â†’ b || b â‰¡ b
||-same {tt} = refl
||-same {ff} = refl

------------------------------------------------------------------------------
-- p. 38 2.4 Theorems with Hypotheses

{-
to express an assumption, write fun that
- takes a proof of assumption
- returns proof of desired result
-}

-- if b1 || b2 is false, then b1 must be false
||â‰¡ffâ‚ : âˆ€ {b1 b2}
       â†’ b1 || b2 â‰¡ ff -- assumption
       â†’ b1       â‰¡ ff -- desired result

-- 1st (implicit) arg is 'ff'
-- 2nd (explicit) arg is ((b1 || b2) â‰¡ ff) bound to 'p' (but not used)
||â‰¡ffâ‚ {ff} p = refl -- b1 = ff â‰¡ ff

-- absurd pattern '()'
||â‰¡ffâ‚ {tt} ()       -- no '=' sign because impossible

{-
To prove the impossible, but only if some impossible assumption is true,
use absurd, since that impossible assumption can never be satisfied by a use of this theorem.
-}

-- p 41 alternative

||â‰¡ffâ‚-2 : âˆ€ {b1 b2} â†’ b1 || b2 â‰¡ ff â†’ b1 â‰¡ ff
||â‰¡ffâ‚-2 {ff} p = refl
||â‰¡ffâ‚-2 {tt} p = p -- 'p' is equal to 'tt â‰¡ ff' -- the desired result of 'b1' instantiated to 'tt'

-- prefer version that uses absurd -- more robust to later changes

------------------------------------------------------------------------------
-- p 42 2.4.3 Matching on equality proofs

{-
special case on CONGRUENCE
if X equals Y then any TYPE containing X is equal to that same TYPE with X's replaced by Y

Congruence holds for definitional equality automatically.
Congruence must be proved for PROPOSITIONAL equalities 'a â‰¡ b'
-}

||-congâ‚ : âˆ€ {b1 b1â€™ b2}        -- implicit args
         â†’ b1       â‰¡ b1â€™       -- explicit arg
         â†’ b1 || b2 â‰¡ b1â€™ || b2 -- desired result
||-congâ‚ refl = refl

{-
-- p 43

only one way to construct an equality proof : via 'refl' constructor

refl can only prove something of the form  x â‰¡ x
- so Agda deduces b1 must be exactly b1â€™

Agda uses definitional
- knows b1 must be definitionally equal to b1â€™
- so refines the desired type using this definitional equality

So only need to prove : ((b1 || b2) â‰¡ (b1 || b2)) -- b1' replaced with b1 since equal
- via 'refl'

------------------------------------------------------------------------------
REFL

Important rule about using type refinements (refl).

Not allowed in such a way that non-variable terms are discovered
 to be definitionally equal to other such terms.

e.g.,

two non-variable terms are definitionally equal:
  b1 || b2
  ff

------------------------------------------------------------------------------
DOT PATTERN

b1, b1â€™, and b2 are implicit arguments above.

To include them in the pattern on the left-hand side of the equation:

||-congâ‚ : âˆ€ {b1 b1â€™ b2}        -- implicit args
         â†’ b1       â‰¡ b1â€™       -- explicit arg
         â†’ b1 || b2 â‰¡ b1â€™ || b2 -- desired result
||-congâ‚ {b1}{b1â€™}{b2} refl = refl

but Agda will complain because to type check this pattern, b1 and b1' can NOT be distinct.
Agda deduces b1 and b1â€™ to be definitionally equal.

Workaround : dot pattern:

||-congâ‚ : âˆ€ {b1 b1â€™ b2}        -- implicit args
         â†’ b1       â‰¡ b1â€™       -- explicit arg
         â†’ b1 || b2 â‰¡ b1â€™ || b2 -- desired result
||-congâ‚ {b1}{.b1}{b2} refl = refl

Writing â€œ.â€ in front of term in pattern tells Agda that term is not a subpattern to match.
Rather it has a form which is dictated by the type of the whole pattern.
-}

------------------------------------------------------------------------------
-- p 44 2.4.4 The REWRITE directive

||-congâ‚‚ : âˆ€ {b1 b2 b2'}
         â†’ b2       â‰¡ b2'
         â†’ b1 || b2 â‰¡ b1 || b2'
||-congâ‚‚ p rewrite p = refl

{-
pattern variable p : with type b2 â‰¡ b2â€™

rewrite every occurrence of the left-hand side,
as it appears in the current goal,
with the right-hand side.

goal is formula to prove on right-hand side of current equation

rewrite p : transform the b2 (the left side of p) in
   b1 || b2  â‰¡ b1 || b2'
to
         b2' (the right side of p)
so goal (the type Agda is checking against the right-hand side of the equation) becomes
   b1 || b2â€™ â‰¡ b1 || b2â€™

REWRITE

given proof 'p' of some equation X â‰¡ Y
(any expression which has X â‰¡ Y as its type, e.g., call to lemma of that type)
look in goal
for any occurrences of X
transform those into Y

X and Y can be complex expressions (not just variables)

------------------------------------------------------------------------------
-- p 44 2.5 Further examples

proving a polymorphic theorem

for every type level â„“
and every type A at that level
and for all booleans
the given ITE holds
-}

ite-same : âˆ€ {â„“} {A : Set â„“}    -- two implicit args
                                --     so no patterns needed on left hand side of equations
         â†’ âˆ€ (b : ğ”¹) (x : A)    -- two explicit args
         â†’ if b then x else x
         â‰¡ x
-- reason by cases on 'b'
ite-same tt _ = refl -- x â‰¡ x
ite-same ff _ = refl

------------------------------------------------------------------------------
-- p 45

B-contra : ff â‰¡ tt           -- if ff â‰¡ tt holds
         â†’ (âˆ€ {P : Set} â†’ P) -- then can prove anything
                             --      every formula P is true (which is NOT true)
B-contra ()

------------------------------------------------------------------------------
-- p 46 SUMMARY

{-
- equality TYPE t â‰¡ tâ€™ expresses equality of expressions t and tâ€™, which must have the same type

- prove equality with refl; will prove t â‰¡ t' for any definitionally equal t and tâ€™

- two exprs definitionally equal if they can be proved equal using their defining equations

- proof is program defined using pattern matching

- Pattern matching can instantiate universally quantified variables which appear in the type.
  Has the effect of specializing the desired formula to the specific instances of those variables.

- Args can be declared implicit with curly braces in the type.
  Can pattern match on implicit arguments,
  using curly braces around the pattern on left-hand side of equation

- assumptions in theorems are args to programs which serve as proofs of those theorems

- absurd pattern can be used when an assumption is definitionally equal to an impossible equality,
  where the equated terms start with different constructors

- When using refl as the pattern for an equality assumption t â‰¡ tâ€™,
  Agda will try to refine the type by making t and tâ€™ definitionally equal.
-}

------------------------------------------------------------------------------
-- p 47 Exercises

-- 1

&&-idem : âˆ€ {b}         -- implicit arg
        â†’ b && b â‰¡ b    -- result
&&-idem {tt} = refl
&&-idem {ff} = refl

||-idem : âˆ€ {b}         -- implicit arg
        â†’ b || b â‰¡ b    -- result
||-idem {tt} = refl
||-idem {ff} = refl

||â‰¡ffâ‚‚ : âˆ€ {b1 b2}      -- implicit args
       â†’ b1 || b2 â‰¡ ff  -- explicit arg
       â†’       b2 â‰¡ ff  -- result
||â‰¡ffâ‚‚ {ff}{ff} _ = refl
{-
||â‰¡ffâ‚‚ {tt} ()
||â‰¡ffâ‚‚ {ff}{tt} ()
-}

||-tt : âˆ€ (b : ğ”¹)       -- explicit arg
      â†’ b || tt â‰¡ tt    -- result
||-tt tt = refl
||-tt ff = refl

ite-arg : âˆ€{â„“ â„“'} {A : Set â„“} {B : Set â„“'}                    -- implicit args
        â†’ (f : A â†’ B) (b : ğ”¹) (x y : A)                       -- explicit args
        â†’ (f (if b then x else y)) â‰¡ (if b then f x else f y) -- result
ite-arg _ tt _ _ = refl
ite-arg _ ff _ _ = refl

ğ”¹-contra : ff â‰¡ tt
         â†’ âˆ€{â„“} {P : Set â„“}
         â†’ P
ğ”¹-contra ()
{-
open import sum
||-split : âˆ€ {b b' : ğ”¹}
         â†’ b || b' â‰¡ tt
         â†’ b â‰¡ tt âŠ b' â‰¡ tt
||-split{tt}{tt} p = injâ‚ refl
||-split{tt}{ff} p = injâ‚ refl
||-split{ff}{tt} p = injâ‚‚ refl
||-split{ff}{ff} ()

ğ”¹-dec : âˆ€ (b : ğ”¹)
      â†’ b â‰¡ tt âŠ b â‰¡ ff
ğ”¹-dec tt = injâ‚ refl
ğ”¹-dec ff = injâ‚‚ refl
-}
&&-snd : {p1 p2 : ğ”¹}    -- implicit args
       â†’ p1 && p2 â‰¡ tt  -- explicit arg
       â†’       p2 â‰¡ tt  -- result
&&-snd {tt} {tt} _ = refl
--&&-snd{ff} ()

&&-fst : {p1 p2 : ğ”¹}
       â†’ p1 && p2 â‰¡ tt
       â†’ p1       â‰¡ tt
&&-fst {tt} {tt} _ = refl
-- &&-fst{ff} ()

&&-combo : {p1 p2 : ğ”¹}         -- implicit
         â†’ p1       â‰¡ tt       -- explcit
         â†’       p2 â‰¡ tt       -- explcit
         â†’ p1 && p2 â‰¡ tt       -- result
&&-combo {tt} {tt} _ _ = refl
{- alternative
&&-combo{tt} pr1 pr2 = pr2
&&-combo{ff} pr1 pr2 = ğ”¹-contra pr1
-}

&&-ff : âˆ€(b : ğ”¹)
      â†’ b && ff â‰¡ ff
&&-ff tt = refl
&&-ff ff = refl

------------------------------------------------------------------------------
-- 2

ff-imp : âˆ€ (b : ğ”¹)
       â†’ ff imp b â‰¡ tt
ff-imp tt = refl
ff-imp ff = refl

imp-tt : âˆ€ (b : ğ”¹)
       â†’ b imp tt â‰¡ tt
imp-tt tt = refl
imp-tt ff = refl

imp-ff : âˆ€ (b : ğ”¹)
       â†’ b imp ff â‰¡ ~ b
imp-ff tt = refl
imp-ff ff = refl

tt-imp : âˆ€ (b : ğ”¹)
       â†’ tt imp b â‰¡ b
tt-imp tt = refl
tt-imp ff = refl

&&-tt : âˆ€ (b : ğ”¹)
      â†’ b && tt â‰¡ b
&&-tt tt = refl
&&-tt ff = refl

||-ff : âˆ€ (b : ğ”¹)
      â†’ b || ff â‰¡ b
||-ff tt = refl
||-ff ff = refl

&&-contra : âˆ€ (b : ğ”¹)
          â†’ b && ~ b â‰¡ ff
&&-contra tt = refl
&&-contra ff = refl

&&-comm : âˆ€ (b1 b2 : ğ”¹)
        â†’ b1 && b2 â‰¡ b2 && b1
&&-comm ff ff = refl
&&-comm ff tt = refl
&&-comm tt ff = refl
&&-comm tt tt = refl

||-comm : âˆ€ (b1 b2 : ğ”¹)
        â†’ b1 || b2 â‰¡ b2 || b1
||-comm ff ff = refl
||-comm ff tt = refl
||-comm tt ff = refl
||-comm tt tt = refl

&&-assoc : âˆ€ (b1 b2 b3 : ğ”¹)
         â†’ b1 && (b2 && b3) â‰¡ (b1 && b2) && b3
&&-assoc ff ff ff = refl
&&-assoc ff ff tt = refl
&&-assoc ff tt ff = refl
&&-assoc ff tt tt = refl
&&-assoc tt ff ff = refl
&&-assoc tt ff tt = refl
&&-assoc tt tt ff = refl
&&-assoc tt tt tt = refl

||-assoc : âˆ€ (b1 b2 b3 : ğ”¹)
         â†’ b1 || (b2 || b3) â‰¡ (b1 || b2) || b3
||-assoc ff ff ff = refl
||-assoc ff ff tt = refl
||-assoc ff tt ff = refl
||-assoc ff tt tt = refl
||-assoc tt ff ff = refl
||-assoc tt ff tt = refl
||-assoc tt tt ff = refl
||-assoc tt tt tt = refl

~-over-&& : âˆ€ (b1 b2 : ğ”¹)
          â†’ ~ ( b1 && b2 ) â‰¡ (~ b1 || ~ b2)
~-over-&& ff ff = refl
~-over-&& ff tt = refl
~-over-&& tt ff = refl
~-over-&& tt tt = refl

~-over-|| : âˆ€ (b1 b2 : ğ”¹)
          â†’ ~ ( b1 || b2 ) â‰¡ (~ b1 && ~ b2)
~-over-|| ff ff = refl
~-over-|| ff tt = refl
~-over-|| tt ff = refl
~-over-|| tt tt = refl

&&-over-||-l : âˆ€ (a b c : ğ”¹)
             â†’ a && (b || c) â‰¡ (a && b) || (a && c)
&&-over-||-l ff ff ff = refl
&&-over-||-l ff ff tt = refl
&&-over-||-l ff tt ff = refl
&&-over-||-l ff tt tt = refl
&&-over-||-l tt ff ff = refl
&&-over-||-l tt ff tt = refl
&&-over-||-l tt tt ff = refl
&&-over-||-l tt tt tt = refl
{-
&&-over-||-r : âˆ€ (a b c : ğ”¹) â†’ (a || b) && c â‰¡ (a && c) || (b && c)
||-over-&&-l : âˆ€ (a b c : ğ”¹) â†’ a || (b && c) â‰¡ (a || b) && (a || c)
||-over-&&-r : âˆ€ (a b c : ğ”¹) â†’ (a && b) || c â‰¡ (a || c) && (b || c)
&&-congâ‚ : âˆ€ {b1 b1' b2 : ğ”¹} â†’ b1 â‰¡ b1' â†’ b1 && b2 â‰¡ b1' && b2
&&-congâ‚‚ : âˆ€ {b1 b2 b2' : ğ”¹} â†’ b2 â‰¡ b2' â†’ b1 && b2 â‰¡ b1 && b2'
&&-intro : âˆ€ {b1 b2 : ğ”¹} â†’ b1 â‰¡ tt â†’ b2 â‰¡ tt â†’ b1 && b2 â‰¡ tt
||-intro1 : âˆ€ {b1 b2 : ğ”¹} â†’ b1 â‰¡ tt â†’ b1 || b2 â‰¡ tt
--&&-elim : âˆ€ {b1 b2 : ğ”¹} â†’ b1 && b2 â‰¡ tt â†’ b1 â‰¡ tt âˆ§ b2 â‰¡ tt
&&-elim1 : âˆ€ {b1 b2 : ğ”¹} â†’ b1 && b2 â‰¡ tt â†’ b1 â‰¡ tt
&&-elim2 : âˆ€ {b1 b2 : ğ”¹} â†’ b1 && b2 â‰¡ tt â†’ b2 â‰¡ tt
--||-elim : âˆ€ {b1 b2 : ğ”¹} â†’ b1 || b2 â‰¡ tt â†’ b1 â‰¡ tt âˆ¨ b2 â‰¡ tt
-}
~-cong : âˆ€ {b b' : ğ”¹}
       â†’   b â‰¡   b'
       â†’ ~ b â‰¡ ~ b'
~-cong refl = refl

ite-congâ‚ : âˆ€{â„“}{A : Set â„“} {b b' : ğ”¹}
            (x y : A)
          â†’     b                â‰¡     b'
          â†’ (if b then x else y) â‰¡ (if b' then x else y)
ite-congâ‚ _ _ refl = refl

ite-congâ‚‚ : âˆ€{â„“} {A : Set â„“}
            (b : ğ”¹)
            {x x' : A}
            (y : A)
          â†’            x         â‰¡            x'
          â†’ (if b then x else y) â‰¡ (if b then x' else y)
ite-congâ‚‚ _ _ refl = refl

ite-congâ‚ƒ : âˆ€{â„“}{A : Set â„“}
            (b : ğ”¹)
            (x : A)
            {y y' : A}
          â†’                   y  â‰¡                   y'
          â†’ (if b then x else y) â‰¡ (if b then x else y')
ite-congâ‚ƒ _ _ refl = refl

--&&-split : âˆ€ {b b' : ğ”¹} â†’ b || b' â‰¡ ff â†’ b â‰¡ ff âŠ b' â‰¡ ff
{-
imp-same : âˆ€ (b : ğ”¹) â†’ b imp b â‰¡ tt
imp-to-|| : âˆ€ (b1 b2 : ğ”¹) â†’ (b1 imp b2) â‰¡ (~ b1 || b2)
imp-mp : âˆ€ {b b' : ğ”¹} â†’ b imp b' â‰¡ tt â†’ b â‰¡ tt â†’ b' â‰¡ tt
imp-antisymm : âˆ€ {b1 b2 : ğ”¹} â†’ b1 imp b2 â‰¡ tt â†’ b2 imp b1 â‰¡ tt â†’ b1 â‰¡ b2
ff-xor : âˆ€ (b : ğ”¹) â†’ ff xor b â‰¡ b
tt-xor : âˆ€ (b : ğ”¹) â†’ tt xor b â‰¡ ~ b
~-xor-distrb : âˆ€ (a b : ğ”¹) â†’ ~ (a xor b) â‰¡ ~ a xor b
xor-distrib-&& : âˆ€ (x y : ğ”¹) â†’ x xor (y && x) â‰¡ ~ y && x
xor~hop : âˆ€ (a b : ğ”¹) â†’ ~ a xor b â‰¡ a xor ~ b
xor-comm : âˆ€ (b1 b2 : ğ”¹) â†’ b1 xor b2 â‰¡ b2 xor b1
xor-assoc : (b1 b2 b3 : ğ”¹) â†’ b1 xor (b2 xor b3) â‰¡ (b1 xor b2) xor b3
xor-anti-idem : (b : ğ”¹) â†’ b xor b â‰¡ ff
xor-â‰¡ : {b1 b2 : ğ”¹} â†’ b1 xor b2 â‰¡ ff â†’ b1 â‰¡ b2
nor-not : âˆ€ (b : ğ”¹) â†’ b nor b â‰¡ ~ b
nor-or : âˆ€ (b1 b2 : ğ”¹) â†’ (b1 nor b2) nor (b1 nor b2) â‰¡ b1 || b2
nor-and : âˆ€ (b1 b2 : ğ”¹) â†’ (b1 nor b1) nor (b2 nor b2) â‰¡ b1 && b2
nor-comm : âˆ€ (b1 b2 : ğ”¹) â†’ b1 nor b2 â‰¡ b2 nor b1
nand-comm : âˆ€ (b1 b2 : ğ”¹) â†’ b1 nand b2 â‰¡ b2 nand b1
-}
------------------------------------------------------------------------------
-- 3

z02-3a : tt â‰¡ tt
z02-3a = refl

z02-3b : ff â‰¡ ff
z02-3b = refl

-- NO z02-3c : ff â‰¡ tt

z02-3d : ff && ff â‰¡ ~ tt
z02-3d = refl

z02-3e : âˆ€ (x : ğ”¹)
       â†’ tt && x
       â‰¡ x
z02-3e _ = refl

z02-3f : âˆ€ (x : ğ”¹)
       â†’ x && tt
       â‰¡ x
z02-3f tt = refl
z02-3f ff = refl


